{
 "cells": [
  {
   "cell_type": "markdown",
   "metadata": {},
   "source": [
    "# Exercise 2.9: Expected Output Changes and Permanent Income\n",
    "\n",
    "Equation  \n",
    "$$\n",
    "y_t - y^p_t = \\sum_{j=1}^{\\infty} \\frac{1}{(1+r)^j} E_t \\Delta y_{t+j}\n",
    "$$  \n",
    "expresses the difference between current and permanent income, $y_t - y^p_t$, as the present discounted value of expected future changes in the endowment.  \n",
    "\n",
    "**Task:**  \n",
    "- Present a step-by-step derivation starting from:  \n",
    "  $$\n",
    "  y^p_t = \\frac{r}{1+r} \\sum_{j=0}^{\\infty} \\frac{E_t y_{t+j}}{(1+r)^j}\n",
    "  $$\n",
    "  and  \n",
    "  $$\n",
    "  \\Delta y_{t+j} = y_{t+j} - y_{t+j-1}\n",
    "  $$\n",
    "- Comment on the cyclical properties of $y_t - y^p_t$ depending on whether the **level** or the **change** of $y_t$ follows an AR(1) process."
   ]
  },
  {
   "cell_type": "markdown",
   "metadata": {},
   "source": [
    "## Step-by-Step Derivation\n",
    "\n",
    "Multiply  \n",
    "$$\n",
    "y^p_t = \\frac{r}{1+r} \\sum_{j=0}^{\\infty} \\frac{E_t y_{t+j}}{(1+r)^j}\n",
    "$$  \n",
    "by $\\frac{1+r}{r}$:  \n",
    "$$\n",
    "\\frac{1+r}{r} y^p_t = \\sum_{j=0}^{\\infty} \\frac{E_t y_{t+j}}{(1+r)^j}\n",
    "$$\n",
    "\n",
    "Split the sum:  \n",
    "$$\n",
    "\\frac{1+r}{r} y^p_t = y_t + \\sum_{j=1}^{\\infty} \\frac{E_t y_{t+j}}{(1+r)^j}\n",
    "$$\n",
    "\n",
    "Subtract $y^p_t$ from both sides:  \n",
    "$$\n",
    "\\frac{1}{r} y^p_t = y_t - y^p_t + \\sum_{j=1}^{\\infty} \\frac{E_t y_{t+j}}{(1+r)^j}\n",
    "$$\n",
    "\n",
    "Rearrange:  \n",
    "$$\n",
    "y_t - y^p_t = - \\sum_{j=1}^{\\infty} \\frac{E_t y_{t+j}}{(1+r)^j} + \\frac{1}{r} y^p_t\n",
    "$$\n",
    "\n",
    "Divide the original $y^p_t$ expression by $r$:  \n",
    "$$\n",
    "\\frac{1}{r} y^p_t = \\sum_{j=0}^{\\infty} \\frac{E_t y_{t+j}}{(1+r)^{j+1}}\n",
    "$$\n",
    "\n",
    "Substitute back:  \n",
    "$$\n",
    "y_t - y^p_t = - \\sum_{j=1}^{\\infty} \\frac{E_t y_{t+j}}{(1+r)^j} + \\sum_{j=0}^{\\infty} \\frac{E_t y_{t+j}}{(1+r)^{j+1}}\n",
    "$$\n",
    "\n",
    "Simplify:  \n",
    "$$\n",
    "y_t - y^p_t = - \\sum_{j=1}^{\\infty} \\frac{1}{(1+r)^j} (E_t y_{t+j} - E_t y_{t+j-1})\n",
    "$$\n",
    "\n",
    "Using $\\Delta y_{t+j} = y_{t+j} - y_{t+j-1}$:  \n",
    "$$\n",
    "y_t - y^p_t = \\sum_{j=1}^{\\infty} \\frac{1}{(1+r)^j} E_t \\Delta y_{t+j}\n",
    "$$\n"
   ]
  },
  {
   "cell_type": "markdown",
   "metadata": {},
   "source": [
    "## Cyclical Properties\n",
    "\n",
    "### Case 1: $y_t$ is AR(1)\n",
    "From:  \n",
    "$$\n",
    "y^p_t = \\frac{r}{1+r-\\rho} y_t\n",
    "$$  \n",
    "we have:  \n",
    "$$\n",
    "y_t - y^p_t = \\frac{1-\\rho}{1+r-\\rho} y_t\n",
    "$$  \n",
    "Since $\\frac{1-\\rho}{1+r-\\rho} > 0$,  \n",
    "$y_t - y^p_t$ is **perfectly procyclical** ($corr(y_t - y^p_t, y_t) = 1$).\n",
    "\n",
    "### Case 2: $\\Delta y_t$ is AR(1)\n",
    "$$\n",
    "E_t \\Delta y_{t+j} = \\rho^j \\Delta y_t\n",
    "$$  \n",
    "so:  \n",
    "$$\n",
    "y_t - y^p_t = -\\frac{\\rho}{1+r-\\rho} \\Delta y_t\n",
    "$$  \n",
    "Since $\\frac{-\\rho}{1+r-\\rho} < 0$,  \n",
    "$y_t - y^p_t$ is **perfectly countercyclical** ($corr(y_t - y^p_t, \\Delta y_t) = -1$).\n"
   ]
  }
 ],
 "metadata": {
  "kernelspec": {
   "display_name": "base",
   "language": "python",
   "name": "python3"
  },
  "language_info": {
   "name": "python",
   "version": "3.9.12"
  }
 },
 "nbformat": 4,
 "nbformat_minor": 2
}
